finish RNDN spec and redesign Lib.Spec

code/mpfr/MPFR.Add.Spec.fst
@@ -3,100 +3,102 @@ module MPFR.Add.Spec
 open FStar.Mul
 open MPFR.Lib.Spec
 
+#set-options "--z3refresh --z3rlimit 5 --max_fuel 1 --initial_fuel 0 --max_ifuel 1 --initial_ifuel 0"
+
 (* Proprieties for addition *)
-val add: a:mpfr_structP{valid_structP a} ->
-         b:mpfr_structP{valid_structP b /\ a.sign = b.sign} ->
-    Tot (r:mpfr_structP{r.sign = a.sign /\ r.exp >= mpfr_EMIN_P /\ mpfr_mp_cond r /\
-          ((a.mant * pow2 (a.exp - mpfr_EMIN_P)) +
-	   (b.mant * pow2 (b.exp - mpfr_EMIN_P)) =
-	   (r.mant * pow2 (r.exp - mpfr_EMIN_P)))})
+val add: a:floating_point ->
+         b:floating_point{a.sign = b.sign} ->
+    Tot (r:floating_point{r.sign = a.sign /\
+          (let elb = min a.exp b.exp in
+	   r.exp >= elb /\
+           (a.mant * pow2 (a.exp - elb)) +
+	   (b.mant * pow2 (b.exp - elb)) =
+	   (r.mant * pow2 (r.exp - elb)))})
 
 (* Implementation for addition *)
 private let min (a:int) (b:int) = if a >= b then b else a
 private let max (a:int) (b:int) = if a >= b then a else b
 
-val add_mant: a:mpfr_structP{valid_structP a} ->
-              b:mpfr_structP{valid_structP b /\ a.sign = b.sign} ->
+val add_mant: a:floating_point ->
+              b:floating_point{a.sign = b.sign} ->
 	  Tot nat
 let add_mant a b =
     if a.exp >= b.exp then a.mant * pow2 (a.exp - b.exp) + b.mant
                      else b.mant * pow2 (b.exp - a.exp) + a.mant
     
-val add_exp : a:mpfr_structP{valid_structP a} ->
-              b:mpfr_structP{valid_structP b /\ a.sign = b.sign} ->
-	 Tot (r:int{r >= mpfr_EMIN_P})
+val add_exp : a:floating_point ->
+              b:floating_point{a.sign = b.sign} ->
+	 Tot (r:int{r >= min a.exp b.exp})
 let add_exp a b = min a.exp b.exp
 
-val add_prec: a:mpfr_structP{valid_structP a} ->
-              b:mpfr_structP{valid_structP b /\ a.sign = b.sign} ->
+val add_prec: a:floating_point ->
+              b:floating_point{a.sign = b.sign} ->
 	  Tot nat
 let add_prec a b =
     let p0 = if a.exp >= b.exp then max (a.prec + a.exp - b.exp) b.prec 
                               else max (b.prec + b.exp - a.exp) a.prec in
     if add_mant a b < pow2 p0 then p0 else p0 + 1
 
-open FStar.Math.Lemmas
 
-val lemma_mult_lt_right: a:pos -> b:nat -> c:nat -> Lemma 
-    (requires b < c)
-    (ensures  b * a < c * a)
-let lemma_mult_lt_right a b c = ()
+open MPFR.Lemmas
 
 (* Useful lemmas *)
-val add_mp_cond_lemma: a:mpfr_structP{valid_structP a} ->
-                       b:mpfr_structP{valid_structP b /\ a.sign = b.sign} ->
+val add_fp_lemma: a:floating_point ->
+                  b:floating_point{a.sign = b.sign} ->
     Lemma (let sp = add_prec a b in
            let sm = add_mant a b in
 	   pow2 (sp - 1) <= sm /\ sm < pow2 sp)
-let add_mp_cond_lemma a b =
+let add_fp_lemma a b =
     let sp = add_prec a b in
     let sm = add_mant a b in
     let p0 = if a.exp >= b.exp then max (a.prec + a.exp - b.exp) b.prec 
                               else max (b.prec + b.exp - a.exp) a.prec in
     if sm < pow2 p0 then begin
 	if a.exp >= b.exp then begin
-	    lemma_mult_le_right (pow2 (a.exp - b.exp)) (pow2 (a.prec - 1)) a.mant;
-	    pow2_plus (a.prec - 1) (a.exp - b.exp)
+	    lemma_mul_le_right (pow2 (a.exp - b.exp)) (pow2 (a.prec - 1)) a.mant;
+	    lemma_pow2_mul (a.prec - 1) (a.exp - b.exp)
 	end else begin
-	    lemma_mult_le_right (pow2 (b.exp - a.exp)) (pow2 (b.prec - 1)) b.mant;
-	    pow2_plus (b.prec - 1) (b.exp - a.exp)
+	    lemma_mul_le_right (pow2 (b.exp - a.exp)) (pow2 (b.prec - 1)) b.mant;
+	    lemma_pow2_mul (b.prec - 1) (b.exp - a.exp)
 	end
     end else begin
 	if a.exp >= b.exp then begin
-	    lemma_mult_lt_right (pow2 (a.exp - b.exp)) a.mant (pow2 a.prec);
-	    pow2_plus a.prec (a.exp - b.exp);
-	    pow2_le_compat (max (a.prec + a.exp - b.exp) b.prec) (a.prec + a.exp - b.exp);
-	    pow2_le_compat (max (a.prec + a.exp - b.exp) b.prec) b.prec;
-	    pow2_double_sum (max (a.prec + a.exp - b.exp) b.prec)
+	    lemma_mul_lt_right (pow2 (a.exp - b.exp)) a.mant (pow2 a.prec);
+	    lemma_pow2_mul a.prec (a.exp - b.exp);
+	    lemma_pow2_le (a.prec + a.exp - b.exp) (max (a.prec + a.exp - b.exp) b.prec);
+	    lemma_pow2_le b.prec (max (a.prec + a.exp - b.exp) b.prec);
+	    lemma_pow2_double (max (a.prec + a.exp - b.exp) b.prec)
 	end else begin
-	    lemma_mult_lt_right (pow2 (b.exp - a.exp)) b.mant (pow2 b.prec);
-	    pow2_plus b.prec (b.exp - a.exp);
-	    pow2_le_compat (max (b.prec + b.exp - a.exp) a.prec) (b.prec + b.exp - a.exp);
-	    pow2_le_compat (max (b.prec + b.exp - a.exp) a.prec) a.prec;
-	    pow2_double_sum (max (b.prec + b.exp - a.exp) a.prec)
+	    lemma_mul_lt_right (pow2 (b.exp - a.exp)) b.mant (pow2 b.prec);
+	    lemma_pow2_mul b.prec (b.exp - a.exp);
+	    lemma_pow2_le (b.prec + b.exp - a.exp) (max (b.prec + b.exp - a.exp) a.prec);
+	    lemma_pow2_le a.prec (max (b.prec + b.exp - a.exp) a.prec);
+	    lemma_pow2_double (max (b.prec + b.exp - a.exp) a.prec)
 	end
     end
 
-val add_value_lemma: a:mpfr_structP{valid_structP a} ->
-                     b:mpfr_structP{valid_structP b /\ a.sign = b.sign} ->
-    Lemma (add_exp a b >= mpfr_EMIN_P /\
-           (a.mant * pow2 (a.exp - mpfr_EMIN_P)) +
-	   (b.mant * pow2 (b.exp - mpfr_EMIN_P)) =
-	   (add_mant a b * pow2 (add_exp a b - mpfr_EMIN_P)))
+val add_value_lemma: a:floating_point ->
+                     b:floating_point{a.sign = b.sign} ->
+    Lemma (let elb = min a.exp b.exp in
+           add_exp a b >= elb /\
+           (a.mant * pow2 (a.exp - elb)) +
+	   (b.mant * pow2 (b.exp - elb)) =
+	   (add_mant a b * pow2 (add_exp a b - elb)))
 let add_value_lemma a b = 
     let sx = add_exp a b in
     let sm = add_mant a b in
+    let elb = min a.exp b.exp in
     if a.exp >= b.exp then begin
-        distributivity_add_left (a.mant * pow2 (a.exp - b.exp)) b.mant (pow2 (sx - mpfr_EMIN_P));
-	paren_mul_right a.mant (pow2 (a.exp - b.exp)) (pow2 (sx - mpfr_EMIN_P));
-	pow2_plus (a.exp - b.exp) (sx - mpfr_EMIN_P)
+        lemma_distr_add_left (a.mant * pow2 (a.exp - b.exp)) b.mant (pow2 (sx - elb));
+	lemma_paren_mul_right a.mant (pow2 (a.exp - b.exp)) (pow2 (sx - elb));
+	lemma_pow2_mul (a.exp - b.exp) (sx - elb)
     end else begin
-        distributivity_add_left (b.mant * pow2 (b.exp - a.exp)) a.mant (pow2 (sx - mpfr_EMIN_P));
-	paren_mul_right b.mant (pow2 (b.exp - a.exp)) (pow2 (sx - mpfr_EMIN_P));
-	pow2_plus (b.exp - a.exp) (sx - mpfr_EMIN_P)
+        lemma_distr_add_left (b.mant * pow2 (b.exp - a.exp)) a.mant (pow2 (sx - elb));
+	lemma_paren_mul_right b.mant (pow2 (b.exp - a.exp)) (pow2 (sx - elb));
+	lemma_pow2_mul (b.exp - a.exp) (sx - elb)
     end
 
 let add a b = 
-    add_mp_cond_lemma a b;
+    add_fp_lemma a b;
     add_value_lemma a b;
     {sign = a.sign; prec = add_prec a b; mant = add_mant a b; exp = add_exp a b}
