code/mpfr/MPFR.Lib.Spec.fst
@@ -1,8 +1,9 @@
 module MPFR.Lib.Spec
 
-(* Pure version of mpfr_struct for internal calculations *)
-(* This struct describe a number: sign * mant * 2^exp    *)
-type mpfr_structP = {
+open FStar.Mul
+
+(* This struct describe a number: sign * mant * 2^exp *)
+type fp_struct = {
     sign: s:int{s = 1 \/ s = -1};
     prec: pos;
     mant: nat;
@@ -10,15 +11,15 @@ type mpfr_structP = {
 }
 
 (* Condition for validity *)
-let mpfr_mp_cond (s:mpfr_structP) = pow2 (s.prec - 1) <= s.mant /\ s.mant < pow2 s.prec
+type floating_point = s:fp_struct{pow2 (s.prec - 1) <= s.mant /\ s.mant < pow2 s.prec}
 
 (* Condition for parameters range corresponding to top level code *)
 let mpfr_PREC_MIN_P = 1
 let mpfr_PREC_MAX_P = 63
 let mpfr_EMIN_P = 1 - pow2 30 - mpfr_PREC_MAX_P
 let mpfr_EMAX_P = pow2 30 - 1 - mpfr_PREC_MIN_P
-let mpfr_range_cond (s:mpfr_structP) =
+let mpfr_range_cond (s:floating_point) =
     mpfr_PREC_MIN_P <= s.prec /\ s.prec <= mpfr_PREC_MAX_P /\
     mpfr_EMIN_P <= s.exp /\ s.exp <= mpfr_EMAX_P
 
-let valid_structP (s:mpfr_structP) = mpfr_mp_cond s /\ mpfr_range_cond s
+type mpfr_fp = f:floating_point{mpfr_range_cond f}
