code/mpfr/MPFR.Rounding.Spec.fst
@@ -1,47 +1,168 @@
 module MPFR.Rounding.Spec
 
+open FStar.Mul
 open FStar.UInt
+open MPFR.Lemmas
 open MPFR.Lib.Spec
 
-(* Definitions of rounding bit and sticky bit *)
-let nth_bit  (#m:pos) (a:uint_t m) (n:nat) = if n < m then nth a n else false
+#set-options "--z3refresh --z3rlimit 5 --max_fuel 1 --initial_fuel 0 --max_ifuel 1 --initial_ifuel 0"
 
-val rb_spec: a:mpfr_structP{valid_structP a} -> p:pos ->
-    Tot (rb:bool{rb = nth_bit #a.prec a.mant p})
-    
-let nth_from (#m:pos) (a:uint_t m) (n:nat) = if n < m then (a % pow2 (m - n) <> 0) else false
+//////////////////////////////////////////////////////////////////////////////////////
+//  RNDN Definition: Rounding to the nearest                                        //
+//  Given floating point number a and precision p, got result r = RNDN(a, p)        //
+//  We should have the following inequality:                                        //
+//  (r.mant - 0.5) * 2 ^ r.exp <= a.mant * 2 ^ a.exp <= (r.mant + 0.5) * 2 ^ r.exp  //
+//  Noting "round to even rule", the inequality should be strict if r.mant % 2 = 1  //
+//////////////////////////////////////////////////////////////////////////////////////
 
-val sb_spec: a:mpfr_structP{valid_structP a} -> p:pos -> 
-    Tot (sb:bool{sb = nth_from #a.prec a.mant (p + 1)})
+let rndn_cond (a:floating_point) (p:pos) (r:floating_point) =
+    let elb = min a.exp r.exp in
+    (r.mant % 2 = 1 ==> ((r.mant * 2 - 1) * pow2 (r.exp - elb) < a.mant * pow2 (a.exp - elb + 1) /\
+                         (r.mant * 2 + 1) * pow2 (r.exp - elb) > a.mant * pow2 (a.exp - elb + 1))) /\
+    (r.mant % 2 = 0 ==> ((r.mant * 2 - 1) * pow2 (r.exp - elb) <= a.mant * pow2 (a.exp - elb + 1) /\
+                         (r.mant * 2 + 1) * pow2 (r.exp - elb) >= a.mant * pow2 (a.exp - elb + 1)))
+
+val rndn_spec: a:floating_point -> p:pos ->
+    Tot (r:floating_point{r.prec = p /\ r.sign = a.sign /\ rndn_cond a p r})
 
 
-(* Useful lemmas for proving rounding/sticky bit proprieties *)		 
+////////////////////////////////////////////////////////////////
+//  Implementation for each rounding mode                     //
+//  Including implementation of rounding/sticky bit for RNDN  //
+////////////////////////////////////////////////////////////////
+
+(* When target precision is larger than before *)
+val rnd_large_p: a:floating_point -> p:pos{p >= a.prec} ->
+    Tot (r:floating_point{r.sign = a.sign /\ r.prec = p /\
+        (let elb = min a.exp r.exp in
+	r.mant * pow2 (r.exp - elb) = a.mant * pow2 (a.exp - elb))})
+	
+let rnd_large_p a p =
+    let elb = min a.exp (a.exp + a.prec - p) in
+    lemma_pow2_mul (p - a.prec) a.prec;
+    lemma_pow2_mul (p - a.prec) (a.prec - 1);
+    lemma_pow2_mul (p - a.prec) (a.exp + a.prec - p - elb);
+    {sign = a.sign; prec = p; mant = a.mant * pow2 (p - a.prec); exp = a.exp + a.prec - p}
+
+(* Getting the first p bits of mantissa *)
+val main_mant: a:floating_point -> p:pos{p < a.prec} -> 
+    Tot (rmant:nat{pow2 (p - 1) <= rmant /\ rmant < pow2 p /\
+        (let rexp = a.exp + a.prec - p in
+	 let elb = min a.exp rexp in
+	 rmant * pow2 (rexp - elb) <= a.mant * pow2 (a.exp - elb) /\
+         a.mant * pow2 (a.exp - elb) < (rmant + 1) * pow2 (rexp - elb))})
+	 
+let main_mant a p =
+    let rexp = a.exp + a.prec - p in
+    let elb = min a.exp rexp in
+    lemma_pow2_div (a.prec - 1) (a.prec - p);
+    lemma_div_le (pow2 (a.prec - 1)) a.mant (pow2 (a.prec - p));
+    lemma_pow2_div_lt a.mant a.prec (a.prec - p);
+    lemma_distr_add_left (a.mant / pow2 (a.prec - p)) 1 (pow2 (rexp - elb));
+    a.mant / pow2 (a.prec - p)
+
+(* Implementation of rounding bit *)
+val rb_spec: a:floating_point -> p:pos -> Tot bool
 let rb_spec a p =
     if a.prec <= p then false
     else nth #a.prec a.mant p
 
+(* Proprieties of rounding bit *)
+val rb_spec_mask_lemma: a:floating_point -> p:pos{p < a.prec} ->
+    Lemma (rb_spec a p = (logand a.mant (pow2_n #a.prec (a.prec - p - 1)) <> 0))
+    
+let rb_spec_mask_lemma a p = 
+    if nth #a.prec a.mant p then 
+        nth_lemma (logand a.mant (pow2_n #a.prec (a.prec - p - 1))) (pow2_n #a.prec (a.prec - p - 1))
+    else 
+        nth_lemma (logand a.mant (pow2_n #a.prec (a.prec - p - 1))) (zero a.prec)
+
+val rb_spec_value_lemma: a:floating_point -> p:pos{p < a.prec} ->
+    Lemma (a.mant % pow2 (a.prec - p) = (if rb_spec a p then pow2 (a.prec - p - 1) else 0) +
+                                        a.mant % pow2 (a.prec - p - 1))
+
+(* Implementation of sticky bit *)
+val sb_spec: a:floating_point -> p:pos -> Tot bool
 let sb_spec a p = 
     if a.prec <= p + 1 then false
     else (a.mant % pow2 (a.prec - (p + 1)) <> 0)
+					
+let rb_spec_value_lemma a p =
+    assert(nth #a.prec a.mant p = nth (shift_right #a.prec a.mant (a.prec - p - 1)) (a.prec - 1));
+    lemma_pow2_mod_div a.mant (a.prec - p) (a.prec - p - 1);
+    lemma_pow2_mod_mod a.mant (a.prec - p) (a.prec - p - 1)
 
-val rb_mask_lemma: #n:pos -> a:uint_t n -> s:nat{s < n} ->
-    Lemma (nth a s = (logand a (pow2_n #n (n - s - 1)) <> 0))
-let rb_mask_lemma #n a s =
-    if nth a s then nth_lemma (logand a (pow2_n #n (n - s - 1))) (pow2_n #n (n - s - 1))
-    else nth_lemma (logand a (pow2_n #n (n - s - 1))) (zero n)
-
-val sb_mask_lemma: #n:pos -> a:uint_t n -> s:pos{s < n} ->
-    Lemma (ensures (nth_from a s = (logand a (pow2_n #n (n - s) - 1) <> 0)))
-let sb_mask_lemma #n a s = 
-    Math.Lemmas.pow2_lt_compat n (n - s);
-    logand_mask #n a (n - s)
-
-
-(* Proprieties of rounding bit and sticky bit *)
-val rb_spec_lemma: a:mpfr_structP{valid_structP a} -> p:pos{p < a.prec} ->
-    Lemma (rb_spec a p = (logand a.mant (pow2_n #a.prec (a.prec - p - 1)) <> 0))
-let rb_spec_lemma a p = rb_mask_lemma #a.prec a.mant p
-
-val sb_spec_lemma: a:mpfr_structP{valid_structP a} -> p:pos{p < a.prec - 1} ->
+(* Proprieties of sticky bit *)
+val sb_spec_mask_lemma: a:floating_point -> p:pos{p < a.prec - 1} ->
     Lemma (sb_spec a p = (logand #a.prec a.mant (pow2_n #a.prec (a.prec - p - 1) - 1) <> 0))
-let sb_spec_lemma a p = sb_mask_lemma #a.prec a.mant (p + 1)
+    
+let sb_spec_mask_lemma a p = 
+    lemma_pow2_lt (a.prec - p - 1) a.prec;
+    logand_mask #a.prec a.mant (a.prec - p - 1)
+
+val sb_spec_value_lemma: a:floating_point -> p:pos{p < a.prec} ->
+    Lemma (sb_spec a p = (a.mant % pow2 (a.prec - p - 1) <> 0))
+    
+let sb_spec_value_lemma a p = ()
+
+
+//////////////////////////////////////////////////////////////
+//  Implementation for RNDN                                 //
+//  3 lemmas for different branches in main implementation  //
+//////////////////////////////////////////////////////////////
+(* Lemmas for RNDN *)
+val rndn_spec_branch1: a:floating_point ->
+    p:pos{p < a.prec /\ (rb_spec a p = false \/ (sb_spec a p = false && main_mant a p % 2 = 0))} ->
+    Tot (r:floating_point{r.prec = p /\ r.sign = a.sign /\ rndn_cond a p r})
+			  
+let rndn_spec_branch1 a p =
+    let rmant = main_mant a p in
+    let rexp = a.exp + a.prec - p in
+    let elb = min a.exp rexp in
+    rb_spec_value_lemma a p;
+    lemma_pow2_mul (a.prec - p) (a.exp - elb + 1);
+    lemma_pow2_mul (a.prec - p - 1) (a.exp - elb + 1);
+    {sign = a.sign; prec = p; mant = rmant; exp = rexp}
+
+val rndn_spec_branch2: a:floating_point -> 
+    p:pos{p < a.prec /\ rb_spec a p = true /\
+         (sb_spec a p = true \/ (sb_spec a p = false /\ main_mant a p % 2 = 1)) /\
+	 main_mant a p + 1 < pow2 p} ->
+    Tot (r:floating_point{r.prec = p /\ r.sign = a.sign /\ rndn_cond a p r})
+
+let rndn_spec_branch2 a p =
+    let rmant = main_mant a p + 1 in
+    let rexp = a.exp + a.prec - p in
+    let elb = min a.exp rexp in
+    rb_spec_value_lemma a p;
+    sb_spec_value_lemma a p;
+    lemma_pow2_mul (a.prec - p) (a.exp - elb + 1);
+    lemma_pow2_mul (a.prec - p - 1) (a.exp - elb + 1);
+    {sign = a.sign; prec = p; mant = rmant; exp = rexp}
+
+val rndn_spec_branch3: a:floating_point -> 
+    p:pos{p < a.prec /\ rb_spec a p = true /\
+         (sb_spec a p = true \/ (sb_spec a p = false /\ main_mant a p % 2 = 1)) /\
+	 main_mant a p + 1 = pow2 p} ->
+    Tot (r:floating_point{r.prec = p /\ r.sign = a.sign /\ rndn_cond a p r})
+
+let rndn_spec_branch3 a p =
+    let rmant = pow2 (p - 1) in
+    let rexp = a.exp + a.prec - p + 1 in
+    let elb = min a.exp rexp in
+    rb_spec_value_lemma a p;
+    sb_spec_value_lemma a p;
+    lemma_pow2_mul (p - 1) 1;
+    lemma_pow2_mul (a.prec - p) (a.exp - elb + 1);
+    lemma_pow2_mul (a.prec - p - 1) (a.exp - elb + 1);
+    {sign = a.sign; prec = p; mant = rmant; exp = rexp}
+
+let rndn_spec a p = 
+    if a.prec <= p then
+        rnd_large_p a p
+    else if rb_spec a p = false || (sb_spec a p = false && main_mant a p % 2 = 0) then 
+        rndn_spec_branch1 a p
+    else if main_mant a p + 1 < pow2 p then
+        rndn_spec_branch2 a p
+    else
+        rndn_spec_branch3 a p
