code/mpfr/MPFR.Lemmas.fst
@@ -1,0 +1,199 @@
+module MPFR.Lemmas
+
+open FStar.Mul
+
+#set-options "--z3refresh --z3rlimit 5 --max_fuel 1 --initial_fuel 0 --max_ifuel 1 --initial_ifuel 0"
+
+(* Nonlinear arithmetic *)
+val lemma_paren_mul_left: a:int -> b:int -> c:int -> Lemma
+    (a * b * c = (a * b) * c)
+
+val lemma_paren_mul_right: a:int -> b:int -> c:int -> Lemma
+    (a * b * c = a * (b * c))
+
+val lemma_mul_le_left: a:nat -> b:int -> c:int -> Lemma
+    (requires (b <= c))
+    (ensures  (a * b <= a * c))
+
+val lemma_mul_le_right: a:nat -> b:int -> c:int -> Lemma
+    (requires (b <= c))
+    (ensures  (b * a <= c * a))
+
+val lemma_mul_lt_left: a:pos -> b:int -> c:int -> Lemma
+    (requires (b < c))
+    (ensures  (a * b < a * c))
+
+val lemma_mul_lt_right: a:pos -> b:int -> c:int -> Lemma
+    (requires (b < c))
+    (ensures  (b * a < c * a))
+
+val lemma_distr_add_left: a:int -> b:int -> c:int -> Lemma
+    ((a + b) * c = a * c + b * c)
+
+val lemma_distr_add_right: a:int -> b:int -> c:int -> Lemma
+    (a * (b + c) = a * b + a * c)
+
+val lemma_distr_sub_left: a:int -> b:int -> c:int -> Lemma
+    ((a - b) * c = a * c - b * c)
+
+val lemma_distr_sub_right: a:int -> b:int -> c:int -> Lemma
+    (a * (b - c) = a * b - a * c)
+
+(* Division and modulo *)
+val lemma_small_div: a:nat -> b:pos -> Lemma
+    (requires (a < b))
+    (ensures  (a / b = 0))
+
+val lemma_small_mod: a:nat -> b:pos -> Lemma
+    (requires (a < b))
+    (ensures  (a % b = a))
+
+val lemma_mul_div: a:nat -> b:pos -> Lemma
+    ((a * b) / b = a)
+
+val lemma_mul_mod: a:nat -> b:pos -> Lemma
+    ((a * b) % b = 0)
+
+val lemma_div_lt: a:nat -> b:nat -> d:pos -> Lemma
+    (requires (a < b /\ b % d = 0))
+    (ensures  (a / d < b / d))
+
+val lemma_div_le: a:nat -> b:nat -> d:pos -> Lemma
+    (requires (a <= b))
+    (ensures  (a / d <= b / d))
+
+val lemma_div_div: a:nat -> b:pos -> c:pos -> Lemma
+    ((a / b) / c = a / (b * c))
+
+val lemma_mod_distr: a:nat -> b:nat -> c:pos -> Lemma
+    ((a + b) % c = (a % c + b % c) % c)
+    
+val lemma_mod_div: a:nat -> b:pos -> c:pos -> Lemma 
+    ((a % (b * c)) / b = (a / b) % c)
+
+val lemma_mod_mod: a:nat -> b:pos -> c:pos -> Lemma
+    ((a % (b * c)) % b = a % b)
+
+(* pow2 proprieties *)
+val lemma_pow2_le: n:nat -> m:nat -> Lemma
+    (requires (n <= m))
+    (ensures  (pow2 n <= pow2 m))
+
+val lemma_pow2_lt: n:nat -> m:nat -> Lemma
+    (requires (n < m))
+    (ensures  (pow2 n < pow2 m))
+    
+val lemma_pow2_mul: n:nat -> m:nat -> Lemma
+    (pow2 n * pow2 m = pow2 (n + m))
+
+val lemma_pow2_small_div: n:nat -> m:nat -> Lemma
+    (requires (n < m))
+    (ensures  (pow2 n / pow2 m = 0))
+
+val lemma_pow2_small_mod: n:nat -> m:nat -> Lemma
+    (requires (n < m))
+    (ensures  (pow2 n % pow2 m = pow2 n))
+
+val lemma_pow2_div: n:nat -> m:nat -> Lemma
+    (requires (m <= n))
+    (ensures  (pow2 n / pow2 m = pow2 (n - m)))
+
+val lemma_pow2_mod: n:nat -> m:nat -> Lemma
+    (requires (m <= n))
+    (ensures  (pow2 n % pow2 m = 0))
+
+val lemma_pow2_double: n:nat -> Lemma
+    (pow2 n + pow2 n = pow2 (n + 1))
+
+val lemma_pow2_div_lt: a:nat -> b:nat -> d:nat -> Lemma
+    (requires (a < pow2 b /\ d <= b))
+    (ensures  (a / pow2 d < pow2 (b - d)))
+    
+val lemma_pow2_mod_div: a:nat -> b:nat -> c:nat -> Lemma
+    (requires (b >= c))
+    (ensures  ((a % pow2 b) / pow2 c = (a / pow2 c) % (pow2 (b - c))))
+
+val lemma_pow2_mod_mod: a:nat -> b:nat -> c:nat -> Lemma
+    (requires (b >= c))
+    (ensures  ((a % pow2 b) % pow2 c = a % pow2 c))
+    
+
+(* Proofs *)
+(* Nonlinear arithmetic *)
+let lemma_paren_mul_left a b c = ()
+let lemma_paren_mul_right a b c = ()
+let lemma_mul_le_left a b c = ()
+let lemma_mul_le_right a b c = ()
+let lemma_mul_lt_left a b c = ()
+let lemma_mul_lt_right a b c = ()
+let lemma_distr_add_left a b c = ()
+let lemma_distr_add_right a b c = ()
+let lemma_distr_sub_left a b c = ()
+let lemma_distr_sub_right a b c = ()
+
+(* Division and modulo *)
+val lemma_euclidean: a:nat -> b:pos -> Lemma
+    (a = (a / b) * b + a % b)
+let lemma_euclidean a b = ()
+val lemma_add_div: a:nat -> n:int -> d:pos -> Lemma
+    (requires (a + n * d >= 0))
+    (ensures  ((a + n * d) / d = a / d + n))
+let lemma_add_div a n d = assert(a / d + n - 1 < (a + n * d) / d /\ (a + n * d) / d < a / d + n + 1)
+val lemma_add_mod: a:nat -> n:int -> d:pos -> Lemma
+    (requires (a + n * d >= 0))
+    (ensures  ((a + n * d) % d = a % d))
+let lemma_add_mod a n d = lemma_add_div a n d
+
+let lemma_small_div a b = ()
+let lemma_small_mod a b = ()
+let lemma_mul_div a b = lemma_add_div 0 a b
+let lemma_mul_mod a b = lemma_mul_div a b
+let lemma_div_lt a b d = assert(a / d >= b / d ==> a >= b)
+let lemma_div_le a b d = lemma_add_div (b - a / d * d) (a / d) d
+
+let lemma_div_div a b c =
+    lemma_euclidean (a / b) c;
+    lemma_add_div (((a / b) % c) * b + a % b) ((a / b) / c) (b * c);
+    lemma_distr_sub_left c 1 b;
+    lemma_small_div (((a / b) % c) * b + a % b) (b * c)
+
+let lemma_mod_distr a b c =
+    lemma_euclidean a c;
+    lemma_add_mod (a % c + b % c) (a / c + b / c) c
+
+let lemma_mod_div a b c =
+    lemma_euclidean a (b * c);
+    lemma_add_div a (- (a / (b * c)) * c) b;
+    assert((a % (b * c)) / b = a / b - (a / (b * c)) * c);
+    lemma_div_div a b c;
+    lemma_euclidean (a / b) c
+
+let lemma_mod_mod a b c =
+    lemma_euclidean a (b * c);
+    lemma_add_mod a (- (a / (b * c)) * c) b
+
+(* pow2 proprieties *)
+let lemma_pow2_le n m = FStar.Math.Lemmas.pow2_le_compat m n
+let lemma_pow2_lt n m = FStar.Math.Lemmas.pow2_lt_compat m n
+let lemma_pow2_mul n m = FStar.Math.Lemmas.pow2_plus n m
+let lemma_pow2_small_div n m =
+    lemma_pow2_lt n m;
+    lemma_small_div (pow2 n) (pow2 m)
+let lemma_pow2_small_mod n m =
+    lemma_pow2_lt n m;
+    lemma_small_mod  (pow2 n) (pow2 m)
+let lemma_pow2_div n m = FStar.Math.Lemmas.pow2_minus n m
+let lemma_pow2_mod n m = 
+    lemma_pow2_mul (n - m) m;
+    lemma_mul_mod (pow2 (n - m)) (pow2 m)
+let lemma_pow2_double n = ()
+let lemma_pow2_div_lt a b d = 
+    lemma_pow2_div b d;
+    lemma_pow2_mod b d;
+    lemma_div_lt a (pow2 b) (pow2 d)
+let lemma_pow2_mod_div a b c =
+    lemma_pow2_mul c (b - c);
+    lemma_mod_div a (pow2 c) (pow2 (b - c))
+let lemma_pow2_mod_mod a b c =
+    lemma_pow2_mul c (b - c);
+    lemma_mod_mod a (pow2 c) (pow2 (b - c))
